

(5.5) Substitution

↑ undoes
(3.4) chain rule

IB M (5.6)

↓
(3.2) Product Rule

Integrating by parts

$$\frac{d}{dx} [f(x)g(x)] = f'(x)g(x) + f(x)g'(x)$$

integrate ↓

$$f(x)g(x) = \int [f'(x)g(x) + f(x)g'(x)] dx$$

$$f(x)g(x) = \int f'(x)g(x) dx + \int f(x)g'(x) dx$$

$$f(x)g(x) - \int g(x)f'(x) dx = \int f(x)g'(x) dx$$

$$\rightarrow \int \underbrace{f(x)}_u \underbrace{g'(x)}_{dv} dx = \underbrace{f(x)}_u \underbrace{g(x)}_v - \int \underbrace{g(x)}_v \underbrace{f'(x)}_{du} dx$$

IF $u = f(x)$ and $dv = g'(x) dx$

↓
 $du = f'(x) dx$

↓
 $v = g(x)$

$$\int u dv = uv - \int v du$$

Ex: $\int x^4 \cos x \, dx$

a) $u = x^4$

$du = 4x^3 \, dx$

$dv = \cos x \, dx$

$v = \sin x$

$\int u \, dv = uv - \int v \, du$

$\int x^4 \cos x \, dx = x^4 \sin x - \int \sin x \cdot 4x^3 \, dx$

↑
degree 3 Poly-
nomial

Integrate
by Parts

↓
Terminates

b) $u = \cos x$

$du = -\sin x \, dx$

$dv = x^4 \, dx$

$v = \frac{1}{5} x^5$

$\int u \, dv = uv - \int v \, du$

$\int \cos x \cdot x^4 \, dx = \frac{1}{5} x^5 \cos x - \int \frac{1}{5} x^5 \cdot -\sin x \, dx$

↑
degree 5 Poly-
nomial

Does not terminate

05/2/2018

Thought process:

1) Do you know this integral?

2) Try a Substitution

3) Integration by Parts.

Ex: Find $\int t e^{-3t} \, dt$.

$u = t$

$du = dt$

$dv = e^{-3t} \, dt$

$v = -\frac{1}{3} e^{-3t}$

$\int u \, dv = u \cdot v - \int v \, du$

$\int t e^{-3t} \, dt = t \cdot -\frac{1}{3} e^{-3t} - \int -\frac{1}{3} e^{-3t} \, dt$

$= -\frac{1}{3} t e^{-3t} + \frac{1}{3} \int e^{-3t} \, dt$

$= -\frac{1}{3} t e^{-3t} - \frac{1}{9} e^{-3t} + C$

$= -\frac{1}{3} e^{-3t} (t + \frac{1}{3}) + C$

-What if it was

a definite integral?

Just evaluate

it on the given

integral.

Ex: Find $\int e^{ax} \cos x \, dx$.

$u = e^{ax}$

$du = a e^{ax} \, dx$

$dv = \cos x \, dx$

$v = \sin x$

$\int u \, dv = u \cdot v - \int v \, du$

$\int e^{ax} \cos x \, dx = e^{ax} \cdot \sin x - \int \sin x \cdot a e^{ax} \, dx$

$= e^{ax} \sin x - a \int e^{ax} \sin x \, dx$

$u = e^{ax}$

$du = a e^{ax} \, dx$

$dv = \sin x \, dx$

$v = -\cos x$

$\int u \, dv = u \cdot v - \int v \, du$

$\int e^{ax} \sin x \, dx = -e^{ax} \cos x - \int -\cos x \cdot a e^{ax} \, dx$

$= -e^{ax} \cos x + a \int e^{ax} \cos x \, dx$

$\int e^{ax} \cos x \, dx = e^{ax} \sin x + a e^{ax} \cos x - a \int e^{ax} \cos x \, dx$

$5 \int e^{ax} \cos x \, dx = e^{ax} \sin x + a e^{ax} \cos x$

$\int e^{ax} \cos x \, dx = \frac{1}{5} e^{ax} \sin x + \frac{a}{5} e^{ax} \cos x + C$